Add I function, clarify bic_aux lemma

Infer.v
@@ -12,16 +12,17 @@ Section timepiece.
 
   Variable Merge : S -> S -> S.
   Variable F : Edge -> S -> S.
+  Variable I : Node -> S.
 
   Definition φ := S -> Prop.
   Definition A := nat -> φ.
 
   (* Computing a new route at a node given routes of its neighbors. *)
-  Definition updated_state (node : Node) (initial : S)
+  Definition updated_state (node : Node)
     (neighbors : list (Node * S)) : S :=
     fold_right (fun (neighbor : (Node * S)) (st : S) =>
                   let (m, ms) := neighbor in
-                  Merge st (F (m, node) ms)) initial neighbors.
+                  Merge st (F (m, node) ms)) (I node) neighbors.
 
   (* The until temporal operator. *)
   Definition until (tau : nat) (before after : φ) : A :=
@@ -56,21 +57,21 @@ Section timepiece.
   (* A helper definition for writing out the inductive condition with times
      erased: all invariants are specified as [S -> Prop] functions. *)
   Definition inductive_condition_untimed
-    (node : Node) (initial : S) (node_invariant : φ)
+    (node : Node) (node_invariant : φ)
     (neighbors : list (Node * S)) (neighbor_invariants : list φ) :=
     length neighbors = length neighbor_invariants ->
     (* if every neighbor's route satisfies the invariant φ *)
     (Forall (fun (c : Node * S * φ) => ((snd c) (snd (fst c)))) (combine neighbors neighbor_invariants)) ->
     (* then the node's invariant holds on the updated state *)
-    (node_invariant (updated_state node initial neighbors)).
+    (node_invariant (updated_state node neighbors)).
 
   (* The original inductive condition for a node [n]. *)
-  Definition inductive_condition (n : Node) (initial : S) (node_invariant : A)
+  Definition inductive_condition (n : Node) (node_invariant : A)
                                  (neighbors : list Node) (neighbor_invariants : list A) :=
     forall (t : nat) (states : list S),
       length states = length neighbors ->
       inductive_condition_untimed
-        n initial (node_invariant (1 + t))
+        n (node_invariant (1 + t))
         (combine neighbors states) (map (fun a => (a t)) neighbor_invariants).
 
   Definition boolean_equals_time_bound (b : bool) (t tau : nat) :=
@@ -126,7 +127,7 @@ Section timepiece.
   Qed.
 
   Definition boolean_inductive_condition
-    (n : Node) (initial : S) (b : bool) (u : Until)
+    (n : Node) (b : bool) (u : Until)
     (neighbors : list Node) (neighbor_invariants : list Until) (B : list bool) :=
       (* associate the booleans with the neighbor witness times *)
       forall (t : nat),
@@ -136,19 +137,20 @@ Section timepiece.
       (forall (states : list S),
           length states = length neighbors ->
           inductive_condition_untimed
-            n initial (buntil b (before u) (after u))
+            n (buntil b (before u) (after u))
             (combine neighbors states)
             (* construct the neighbor invariants with booleans *)
             (map (fun p => buntil (fst p) (before (snd p)) (after (snd p))) (combine B neighbor_invariants))).
 
+  (** Proof that the inductive condition implies the boolean inductive condition. *)
   Lemma ind_vc_until_implies_boolean_ind_vc :
-    forall (n : Node) (initial : S) (b : bool) (tau : nat) (node_before node_after : φ)
+    forall (n : Node) (b : bool) (tau : nat) (node_before node_after : φ)
       (neighbors : list Node) (neighbor_invariants : list Until) (B : list bool),
       length neighbors = length neighbor_invariants ->
-        length B = length neighbor_invariants ->
-      inductive_condition n initial (until tau node_before node_after)
+      length B = length neighbor_invariants ->
+      inductive_condition n (until tau node_before node_after)
         neighbors (map construct_until neighbor_invariants) ->
-      boolean_inductive_condition n initial b (mkUntil tau node_before node_after)
+      boolean_inductive_condition n b (mkUntil tau node_before node_after)
         neighbors neighbor_invariants B.
   Proof.
     unfold
@@ -156,7 +158,7 @@ Section timepiece.
       boolean_inductive_condition,
       booleans_are_time_bounds.
     simpl.
-    intros n initial b tau' node_before node_after.
+    intros n b tau' node_before node_after.
     intros neighbors neighbor_invariants B Hnbrlen Hblen Hindvc t Hnbr_bounds Hn_bound states Hstateslen.
     (* match up the until and buntil *)
     apply (until_has_equivalent_buntil _ _ _ node_before node_after) in Hn_bound.
@@ -169,25 +171,22 @@ Section timepiece.
     assumption.
   Qed.
 
+  (** Proof that the boolean inductive condition implies the inductive condition
+      when the premises of the boolean inductive condition are met.
+   *)
   Lemma boolean_ind_vc_until_implies_ind_vc_aux :
-    forall n initial b tau' before' after' neighbors neighbor_invariants B t,
+    forall n b tau' before' after' neighbors neighbor_invariants B t,
       length B = length neighbor_invariants ->
       booleans_are_time_bounds (combine B (map tau neighbor_invariants)) t ->
       boolean_equals_time_bound b (Datatypes.S t) tau' ->
-      (forall (states : list S),
-          length states = length neighbors ->
-          inductive_condition_untimed n initial (buntil b before' after')
-            (combine neighbors states)
-            (* construct the neighbor invariants with booleans *)
-            (map (fun p => buntil (fst p) (before (snd p)) (after (snd p))) (combine B neighbor_invariants))) ->
+      boolean_inductive_condition n b (mkUntil tau' before' after') neighbors neighbor_invariants B ->
       forall states : list S,
         length states = length neighbors ->
-        inductive_condition_untimed n initial (until tau' before' after' (1 + t)) (combine neighbors states)
+        inductive_condition_untimed n (until tau' before' after' (1 + t)) (combine neighbors states)
           (map (fun x : Until => construct_until x t) neighbor_invariants).
     Proof.
       intros.
-      specialize (H2 states).
-      apply H2 in H3.
+      apply (H2 t H0 H1 states) in H3.
       rewrite (untils_have_equivalent_buntils neighbor_invariants B t); try congruence.
       rewrite (until_has_equivalent_buntil b).
       2: { simpl. assumption. }
